\documentclass[../../main.tex]{subfiles}

\begin{document}

  \begin{shaded}
    Let $A$ and $B$ be $n \times n$ real matrices such that
    $$
    \rank{(AB - BA + I)} = 1
    $$

    where $I$ is the $n \times n$ identity matrix. Prove that
    $$
    \tr{(ABAB)} - \tr{(A^2 B^2)} = \frac{1}{2} n (n - 1)
    $$
  \end{shaded}

  \textbf{Solution:}

  Using some properties of the trace of the product of two matrices, for instance $\tr{(XY)} = \tr{(YX)}$ and $\tr{(X)} + \tr{(Y)} = \tr{(X + Y)}$, the expression to be proven is the same as:
  \begin{equation*}
    \begin{split}
      &
      \tr{(ABAB)} - \tr{(A^2 B^2)} = \\ & \qquad =
      \frac{1}{2}\left(2 \, \tr{(ABAB)} - 2 \, \tr{(A^2 B^2)}\right) = \\ & \qquad =
      \frac{1}{2}\left(\tr{(ABAB)} + \tr{(ABAB)} - \tr{(AABB)} - \tr{(AABB)}\right) = \\ & \qquad =
      \frac{1}{2}\left(\tr{(ABAB)} + \tr{(A(BAB))} - \tr{(A(ABB))} - \tr{((AAB)B)}\right) = \\ & \qquad =
      \frac{1}{2}\left(\tr{(ABAB)} + \tr{((BAB)A)} - \tr{((ABB)A)} - \tr{(B(AAB))}\right) = \\ & \qquad =
      \frac{1}{2}\left(\tr{(ABAB)} + \tr{(BABA)} - \tr{(ABBA)} - \tr{(BAAB)}\right) = \\ & \qquad =
      \frac{1}{2}\tr{(ABAB + BABA - ABBA - BAAB)} = \\ & \qquad =
      \frac{1}{2}\tr{((AB - BA)^2)\qquad }
    \end{split}
  \end{equation*}

  Let $M = AB - BA + I$ and $N = M - I = AB - BA$.

  From the condition $\rank{(M)} = \rank{(AB - BA + I)} = 1$, it is obtained that all eigenvalues of $M$ are zero with multiplicity $n - 1$, or there exists a unique eigenvalue that is non-zero (with multiplicity $1$ and the rest are null eigenvalues with multiplicity $n - 1$).

  As it happens that
  \begin{equation*}
    \begin{split}
      \tr{(M)} & =
      \tr{(AB - BA + I)} = \\ & =
      \tr{(AB)} - \tr{(BA)} + \tr{(I)} = \\ & =
      \tr{(I)} = n
    \end{split}
  \end{equation*}

  then $M$ has a unique non-zero eigenvalue with value $n$, and the rest are null eigenvalues. Hence, the spectrum of the matrix $M$ is $\sigma(M) = \{0, n\}$.

  Since $N = M - I$, the spectrum of $N$ is $\sigma(N) = \{-1, n - 1\}$, and the spectrum of $N^2$ is $\sigma(N^2) = \{1, (n - 1)^2\}$.

  Notice that $\tr{(ABAB)} - \tr{(A^2 B^2)} = \frac{1}{2}\tr{((AB - BA)^2)} = \frac{1}{2}\tr{(N^2)}$. Ant it is known that the trace of $N^2$ is the sum of its eigenvalues, namely:
  $$
  \tr{(N^2)} = 1 \cdot (n - 1) + (n - 1)^2 = n (n - 1)
  $$

  An hence, it is proven that:
  $$
  \tr{(ABAB)} - \tr{(A^2 B^2)} = \frac{1}{2}\tr{((AB - BA)^2)} = \frac{1}{2}\tr{(N^2)} = \frac{1}{2} n (n - 1)
  $$

\end{document}
