\documentclass[../../main.tex]{subfiles}

\begin{document}

  \begin{shaded}
    Suppose that in a not necessarily commutative ring $R$ the square of any element is $0$. Prove that $abc + abc = 0$ for any three elements $a, b, c$.
  \end{shaded}

  \textbf{Solution:}

  Initially it can be seen that $(a + b)^2 = 0$, then $(a + b)^2 = a^2 + ab + ba + b^2 = ab + ba = 0$, where it follows that $ab = - (ba)$.

  Once having this, then
  \begin{equation*}
    \begin{split}
      abc & = a (bc) \\ & =
      - ((bc) a) \\ & =
      - (b (ca)) \\ & =
      (ca) b \\ & =
      c (ab) \\ & =
      - ((ab) c) \\ & =
      - abc
    \end{split}
  \end{equation*}

  And therefore, $abc + abc = 0$.

\end{document}
